preast.check_type

ExtParser/AST.lean
@@ -25,14 +25,230 @@ namespace AST
     | ε : Wellformed (.ε s e)
     | any : Wellformed (.any s e x)
     | terminal : Wellformed (.terminal s e a x)
-    | nonTerminal : ¬SkipPreAST' T → Wellformed (.nonTerminal s e A T)
-    | seq : ¬SkipPreAST' T1 →  Wellformed (.seq s e T1 T2)
-    | prior : ¬SkipPreAST' T1 →  Wellformed (.prior s e T1 T2)
-    | star : ¬SkipPreAST' T0 → (SkipPreAST' TS ∨ StarPreAST' TS) → Wellformed (.star s e T0 TS)
-    | notP : ¬SkipPreAST' T → Wellformed (.notP s e T)
+    | nonTerminal : Wellformed T → ¬SkipPreAST' T → Wellformed (.nonTerminal s e A T)
+    | seq : Wellformed T1 → Wellformed T2 → ¬SkipPreAST' T1 → Wellformed (.seq s e T1 T2)
+    | prior : Wellformed T1 → Wellformed T2 → ¬SkipPreAST' T1 → Wellformed (.prior s e T1 T2)
+    | star : Wellformed T0 → Wellformed TS → ¬SkipPreAST' T0 → (SkipPreAST' TS ∨ StarPreAST' TS) → Wellformed (.star s e T0 TS)
+    | notP : Wellformed T → ¬SkipPreAST' T → Wellformed (.notP s e T)
+
+  def PreAST'.size (T : PreAST' n b) : Nat :=
+    match T with
+    | .skip _ _ _ => 0
+    | .ε _ _ => 0
+    | .any _ _ _ => 0
+    | .terminal _ _ _ _ => 0
+    | .nonTerminal _ _ _ T => T.size + 1
+    | .seq _ _ T1 T2 => T1.size + T2.size + 1
+    | .prior _ _ T1 T2 => T1.size + T2.size + 1
+    | .star _ _ T0 TS => T0.size + TS.size + 1
+    | .notP _ _ T => T.size + 1
   
+
   structure PreAST (n : Nat) (b : Nat) where
     T : PreAST' n b
     wf_T : PreAST'.Wellformed T
+
+  mutual
+
+  inductive SuccessAST : PreAST n b → Prop where
+    | ε : s = e → SuccessAST { T := .ε s e, wf_T := .ε }
+    | any : s.inbound_succ h = e → SuccessAST { T := .any s e x, wf_T := .any }
+    | terminal : s.inbound_succ h = e → a = x → SuccessAST { T := .terminal s e a x, wf_T := .terminal }
+    | nonTerminal : SuccessAST T → SuccessAST { T := .nonTerminal s e A T.T, wf_T := .nonTerminal T.wf_T h}
+    | seq : SuccessAST T1 → SuccessAST T2 → SuccessAST { T := .seq s e T1.T T2.T, wf_T := .seq T1.wf_T T2.wf_T h }
+    | prior_S : ∀ {T2 : PreAST n b}, SuccessAST T1 → SuccessAST { T := .prior s e T1.T T2.T, wf_T := .prior T1.wf_T T2.wf_T h }
+    | prior_FS : FailureAST T1 → SuccessAST T2 → SuccessAST { T := .prior s e T1.T T2.T, wf_T := .prior T1.wf_T T2.wf_T h }
+    | star_F : ∀ {TS : PreAST n b} {h2 : SkipPreAST' TS.T ∨ StarPreAST' TS.T}, FailureAST T0 → SuccessAST { T := .star s e T0.T TS.T, wf_T := .star T0.wf_T TS.wf_T h1 h2 }
+    | star_SS : SuccessAST T0 → SuccessAST TS → SuccessAST { T := .star s e T0.T TS.T, wf_T := .star T0.wf_T TS.wf_T h1 h2 }
+    | notP : FailureAST T → SuccessAST { T := .notP s e T.T, wf_T := .notP T.wf_T h }
+
+  inductive FailureAST : PreAST n b → Prop where
+    | any : s = e → FailureAST { T := .any s e x, wf_T := .any }
+    | terminal_mismatch : s.inbound_succ h = e → a ≠ x → FailureAST { T := .terminal s e a x, wf_T := .terminal }
+    | terminal_empty : s = e → FailureAST { T := .terminal s e a x, wf_T := .terminal }
+    | nonTerminal : FailureAST T → FailureAST { T := .nonTerminal s e A T.T, wf_T := .nonTerminal T.wf_T h}
+    | seq_F : ∀ {T2 : PreAST n b}, FailureAST T1 → FailureAST { T := .seq s e T1.T T2.T, wf_T := .seq T1.wf_T T2.wf_T h }
+    | seq_SF : SuccessAST T1 → FailureAST T2 → FailureAST { T := .seq s e T1.T T2.T, wf_T := .seq T1.wf_T T2.wf_T h }
+    | prior : FailureAST T1 → FailureAST T2 → FailureAST { T := .prior s e T1.T T2.T, wf_T := .prior T1.wf_T T2.wf_T h }
+    | notP : SuccessAST T → FailureAST { T := .notP s e T.T, wf_T := .notP T.wf_T h }
+
+  end
+
+  theorem SuccessAST.ne_failure : ∀ {T : PreAST n b}, SuccessAST T → ¬FailureAST T := by
+    intro T hs hf;
+    match T with
+    | .mk T wf_T => match T with
+      | .skip _ _ _ => cases hs;
+      | .ε _ _ => cases hf;
+      | .any _ _ _ => cases hs; cases hf; apply absurd (by assumption); apply Fin.ne_of_val_ne; apply Nat.ne_of_lt; apply Fin.lt_from_inbound_succ; assumption;
+      | .terminal s e a x => cases hs; cases hf; contradiction; apply absurd (by assumption); apply Fin.ne_of_val_ne; apply Nat.ne_of_lt; apply Fin.lt_from_inbound_succ; assumption;
+      | .nonTerminal s e A _ => match hs with
+        | .nonTerminal (T := Ts) st =>
+          {
+            match Ts with
+            | .mk Ts' _ => simp at hf; match hf with
+              | .nonTerminal (T := Ts) ft => 
+                {
+                  have _ : PreAST'.size Ts.T < PreAST'.size (PreAST'.nonTerminal s e A Ts.T) := by
+                  {
+                    rw [PreAST'.size]; apply Nat.lt_succ_self;
+                  }
+                  apply absurd ft; apply ne_failure; exact st;
+                }
+          }
+      | .seq s e _ _ => match hs with
+        | .seq (T1 := T1) (T2 := T2) st1 st2 =>
+          {
+            match T1, T2 with
+            | .mk T1' _, .mk T2' _ => simp at hf; match hf with
+              | .seq_F (T1 := T1) (T2 := T2) ft1 =>
+                {
+                  have _ : PreAST'.size T1.T < PreAST'.size (PreAST'.seq s e T1.T T2.T) := by
+                  {
+                    rw [PreAST'.size];
+                    apply Nat.lt_succ_of_le; simp;
+                    apply Nat.le_add_right;
+                  }
+                  apply absurd ft1; apply ne_failure; exact st1;
+                }
+              | .seq_SF (T1 := T1) (T2 := T2) _ ft2 =>
+                {
+                  have _ : PreAST'.size T2.T < PreAST'.size (PreAST'.seq s e T1.T T2.T) := by
+                  {
+                    rw [PreAST'.size];
+                    apply Nat.lt_succ_of_le; simp;
+                    apply Nat.le_add_left;
+                  }
+                  apply absurd ft2; apply ne_failure; exact st2;
+                }
+          }
+      | .prior s e _ _ => match hf with
+        | .prior (T1 := T1) (T2 := T2) ft1 ft2 =>
+          {
+            match T1, T2 with
+            | .mk T1' _, .mk T2' _ => simp at hs; match hs with
+              | .prior_S (T1 := T1) (T2 := T2) st1 =>
+                {
+                  have _ : PreAST'.size T1.T < PreAST'.size (PreAST'.prior s e T1.T T2.T) := by
+                  {
+                    rw [PreAST'.size];
+                    apply Nat.lt_succ_of_le; simp;
+                    apply Nat.le_add_right;
+                  }
+                  apply absurd ft1; apply ne_failure; exact st1;
+                }
+              | .prior_FS (T1 := T1) (T2 := T2) _ st2 =>
+                {
+                  have _ : PreAST'.size T2.T < PreAST'.size (PreAST'.prior s e T1.T T2.T) := by
+                  {
+                    rw [PreAST'.size];
+                    apply Nat.lt_succ_of_le; simp;
+                    apply Nat.le_add_left;
+                  }
+                  apply absurd ft2; apply ne_failure; exact st2;
+                }
+          }
+      | .star s e _ _ => cases hf;
+      | .notP s e _ => match hs with
+        | .notP (T := T) ft =>
+          {
+            match T with
+            | .mk T' _ => simp at hf; match hf with
+              | .notP (T := T) st =>
+                {
+                  have _ : PreAST'.size T.T < PreAST'.size (PreAST'.notP s e T.T) := by
+                  {
+                    rw [PreAST'.size];
+                    apply Nat.lt_succ_of_le; simp;
+                  }
+                  apply absurd ft; apply ne_failure; exact st;
+                }
+          }
+  termination_by SuccessAST.ne_failure T _ _ => T.T.size
+
+  theorem FailureAST.ne_success : ∀ {T : PreAST n b}, FailureAST T → ¬SuccessAST T := by
+    intro T hf hs;
+    exact SuccessAST.ne_failure hs hf;
+
+  inductive TypeAST : PreAST n b → Prop
+    | success : SuccessAST T → TypeAST T
+    | failure : FailureAST T → TypeAST T
+    | undefined : ¬SuccessAST T → ¬FailureAST T → TypeAST T
   
+  def PreAST.check_type (T : PreAST n b) : TypeAST T :=
+    match T with
+    | .mk T wf_T => match T with
+      | .skip s e G => .undefined (by intro h; cases h;) (by intro h; cases h;)
+      | .ε s e => match decEq s e with
+        | isTrue heq => .success (.ε heq)
+        | isFalse hne => .undefined (by intro h; cases h; contradiction) (by intro h; cases h;)
+      | .any s e x => match decEq s e, decEq s.val.succ b with
+        | isTrue heq_e, _ => .failure (.any heq_e)
+        | isFalse hne_e, isTrue heq_b => .undefined (by intro h; cases h; contradiction;) (by intro h; cases h; contradiction)
+        | isFalse hne_e, isFalse hne_b => match decEq (s.inbound_succ hne_b) e with
+          | isTrue g => .success (.any g)
+          | isFalse g => .undefined (by intro h; cases h; apply absurd _ g; simp [Fin.inbound_succ] at *; apply Fin.eq_of_val_eq; apply Fin.val_eq_of_eq; assumption) (by intro h; cases h; contradiction;)
+      | .terminal s e a x => match decEq s e, decEq s.val.succ b, decEq a x with
+        | isTrue heq_e, _, _ => .failure (.terminal_empty heq_e)
+        | isFalse hne_e, isTrue heq_b, _ => .undefined (by intro h; cases h; contradiction;) (by intro h; cases h; contradiction; contradiction;)
+        | isFalse hne_e, isFalse hne_b, isTrue heq_ax => match decEq (s.inbound_succ hne_b) e with
+          | isTrue g => .success (.terminal g heq_ax)
+          | isFalse g => .undefined (by intro h; cases h; apply absurd _ g; simp [Fin.inbound_succ] at *; apply Fin.eq_of_val_eq; apply Fin.val_eq_of_eq; assumption) (by intro h; cases h; contradiction; contradiction;)
+        | isFalse hne_e, isFalse hne_b, isFalse hne_ax => match decEq (s.inbound_succ hne_b) e with
+          | isTrue g => .failure (.terminal_mismatch g hne_ax)
+          | isFalse g => .undefined (by intro h; cases h; contradiction;) (by intro h; cases h; apply absurd _ g; simp [Fin.inbound_succ] at *; apply Fin.eq_of_val_eq; apply Fin.val_eq_of_eq; assumption; contradiction;)
+      | .nonTerminal s e A sub_T => match wf_T with
+        | .nonTerminal wf ns =>
+          let T_ast : PreAST n b := (PreAST.mk sub_T wf);
+          have g : (¬SkipPreAST' T_ast.T) := by simp; exact ns;
+          match check_type T_ast with
+          | .success h => .success (.nonTerminal (h := g) h)
+          | .failure h => .failure (.nonTerminal (h := g) h)
+          | .undefined hs hf => .undefined (by intro h; cases h; contradiction;) (by intro h; cases h; contradiction;)
+      | .seq s e T1 T2 => match wf_T with
+        | .seq wf1 wf2 ns =>
+          let T1_ast : PreAST n b := (PreAST.mk T1 wf1);
+          let T2_ast : PreAST n b := (PreAST.mk T2 wf2);
+          have g : (¬SkipPreAST' T1_ast.T) := by simp; exact ns;
+          match check_type T1_ast, check_type T2_ast with
+          | .undefined h1s h1f, _ => .undefined (by intro h; cases h; contradiction;) (by intro h; cases h; contradiction; contradiction;)
+          | .success h1, .success h2 => .success (.seq (h := g) h1 h2)
+          | .success h1, .failure h2 => .failure (.seq_SF (h := g) h1 h2)
+          | .success h1, .undefined h2s h2f => .undefined (by intro h; cases h; contradiction;) (by intro h; cases h; {apply absurd _ (h1.ne_failure); assumption}; {apply absurd _ h2f; assumption})
+          | .failure h1, _ => .failure (.seq_F (T2 := T2_ast) (h := g) h1)
+      | .prior s e T1 T2 => match wf_T with
+        | .prior wf1 wf2 ns =>
+          let T1_ast : PreAST n b := (PreAST.mk T1 wf1);
+          let T2_ast : PreAST n b := (PreAST.mk T2 wf2);
+          have g : (¬SkipPreAST' T1_ast.T) := by simp; exact ns;
+          match check_type T1_ast, check_type T2_ast with
+          | .undefined h1s h1f, _ => .undefined (by intro h; cases h; contradiction; contradiction;) (by intro h; cases h; contradiction;)
+          | .success h1, _ => .success (.prior_S (T2 := T2_ast) (h := g) h1)
+          | .failure h1, .success h2 => .success (.prior_FS (h := g) h1 h2)
+          | .failure h1, .failure h2 => .failure (.prior (h := g) h1 h2)
+          | .failure h1, .undefined h2s h2f => .undefined (by intro h; cases h; apply absurd _ (h1.ne_success); assumption; apply absurd _ h2s; assumption) (by intro h; cases h; apply absurd _ h2f; assumption)
+      | .star s e T0 TS => match wf_T with
+        | .star wf0 wfS n0 nS =>
+          let T0_ast : PreAST n b := (PreAST.mk T0 wf0);
+          let TS_ast : PreAST n b := (PreAST.mk TS wfS);
+          have g1 : (¬SkipPreAST' T0_ast.T) := by simp; exact n0;
+          have g2 : SkipPreAST' TS_ast.T ∨ StarPreAST' TS_ast.T := by 
+          {
+            cases nS; simp; apply Or.inl; assumption; simp; apply Or.inr; assumption;
+          }
+          match check_type T0_ast, check_type TS_ast with
+          | .undefined h1s h1f, _ => .undefined (by intro h; cases h; apply absurd _ h1f; assumption; apply absurd _ h1s; assumption) (by intro h; cases h;)
+          | .failure h0, _ => .success (.star_F (TS := TS_ast) (h1 := g1) (h2 := g2) h0)
+          | .success h0, .success hs => .success (.star_SS (TS := TS_ast) (h1 := g1) (h2 := g2) h0 hs)
+          | .success h0, .failure hs => .undefined (by intro h; cases h; apply absurd _ h0.ne_failure; assumption; apply absurd _ hs.ne_success; assumption) (by intro h; cases h;)
+          | .success h0, .undefined h2s h2f => .undefined (by intro h; cases h; apply absurd _ h0.ne_failure; assumption; contradiction) (by intro h; cases h;)
+      | .notP s e sub_T => match wf_T with
+        | .notP wf ns =>
+          let T_ast : PreAST n b := (PreAST.mk sub_T wf);
+          have g : (¬SkipPreAST' T_ast.T) := by simp; exact ns;
+          match check_type T_ast with
+          | .success h => .failure (.notP (h := g) h)
+          | .failure h => .success (.notP (h := g) h)
+          | .undefined hs hf => .undefined (by intro h; cases h; contradiction) (by intro h; cases h; contradiction)
+
 end AST
